Safe malloc - WIP

theories/examples/safe_malloc.v
@@ -1,6 +1,7 @@
 From iris.algebra Require Import frac.
 From iris.proofmode Require Import tactics.
 From cap_machine Require Import logrel addr_reg_sample fundamental rules proofmode.
+From cap_machine.examples Require Import static_spinlock.
 
 (* A toy malloc implementation *)
 
@@ -16,93 +17,28 @@ From cap_machine Require Import logrel addr_reg_sample fundamental rules proofmo
    This is obviously not very realistic, but is good enough for our simple case
    studies. *)
 
+
 Section SimpleMalloc.
   Context {Σ:gFunctors} {memg:memG Σ} {regg:regG Σ}
-          `{MP: MachineParameters}.
-
-  (* r0 contains the capability pointing to the lock address *)
-  Definition spinlock_instrs' r0 r1 r2 r3 :=
-    encodeInstrsW [
-     Mov r1 1  ; (* value to acquire the lock *)
-     Mov r2 PC ; (* Adresse loop to wait --> label loop*)
-     Lea r2 2  ;
-     (* loop: *)
-     Mov r3 0  ; (* value to check lock state *)
-     CAS r0 r3 r1;
-     Jnz r2 r3
-     (* if (r1 -> 0), then the lock was free, we can continue *)
-     (* if (r1 -> 1), then the lock was locked, we can wait and loop *)
-      ].
-
-  (* Ltac  *)
+          `{lockG Σ, MP: MachineParameters}.
 
   Ltac iInstr_inv Hinv :=
     wp_instr
     ; iInv Hinv as ">Hprog" "Hcls"
-    ; codefrag_facts "Hprog"
+    ; codefrag_facts "Hprog" (* TODO fix this, because it duplicates the hypothesis *)
     ; iInstr "Hprog"
-    ; iMod ("Hcls" with "Hprog") as "_"
-    ; iModIntro ; wp_pure.
+    ; try (match goal with
+           | h: _ |- isCorrectPC _ => apply isCorrectPC_intro; [solve_addr| auto]
+           end)
+    ; try (match goal with
+           | h: _ |- isCorrectPC _ => apply isCorrectPC_intro; [admit| auto]
+           end)
+    ; try (iMod ("Hcls" with "Hprog") as "_" ; iModIntro ; wp_pure).
 
-  (* TODO : now, encapsulate the codefrag in an invariant *)
-  Lemma spinlock_spec (i : CoreN)
-    p_pc b_pc e_pc a_spinlock
-    r0 r1 r2 r3
-    w1 w2 w3
-    p_lock b_lock e_lock a_lock
-    ls
-    N E φ :
-
-    let e_spinlock := (a_spinlock ^+ length (spinlock_instrs' r0 r1 r2 r3))%a in
-
-    ExecPCPerm p_pc ->
-    SubBounds b_pc e_pc a_spinlock e_spinlock ->
-
-    writeAllowed p_lock = true ->
-    withinBounds b_lock e_lock a_lock = true ->
-
-    ↑N ⊆ E ->
-    ⊢ ( inv N (codefrag a_spinlock (spinlock_instrs' r0 r1 r2 r3))
-        ∗ (i, PC) ↦ᵣ WCap p_pc b_pc e_pc a_spinlock
-        ∗ (i, r0) ↦ᵣ (WCap p_lock b_lock e_lock a_lock)
-        ∗ (i,r1) ↦ᵣ w1
-        ∗ (i,r2) ↦ᵣ w2
-        ∗ (i,r3) ↦ᵣ w3
-        ∗ a_lock ↦ₐ ls
-        ∗ ▷ ( (i,PC) ↦ᵣ WCap p_pc b_pc e_pc e_spinlock
-              ∗ (i,r0) ↦ᵣ (WCap p_lock b_lock e_lock a_lock)
-              ∗ (i,r1) ↦ᵣ WInt 1
-              ∗ (∃ w2, (i,r2) ↦ᵣ w2)
-              ∗ (i, r3) ↦ᵣ WInt 0
-              ∗ a_lock ↦ₐ WInt 1
-              -∗
-                WP (i, Seq (Instr Executable)) @ E {{ φ }}
-            )
-        -∗ WP (i, Seq (Instr Executable)) @ E {{ φ }})%I.
-  Proof.
-    intro e_spinlock.
-    iIntros (HPC_exec HPC_bounds Hwrite_lock Hwrite_bounds HN)
-      "(#Hinv_prog & HPC & Hr0 & Hr1 & Hr2 & Hr3 & Hb_lock & Hφ)".
-
-    do 3 (iInstr_inv "Hinv_prog").
-    iLöb as "IH" forall (w3 ls).
-    iInstr_inv "Hinv_prog".
-    destruct (decide ( ls = WInt 0 )).
-    - subst.
-      do 2 (iInstr_inv "Hinv_prog").
-      iApply "Hφ". iFrame.
-      iExists _ ; iFrame.
-    - do 2 (iInstr_inv "Hinv_prog").
-      iAssert ( (i, PC) ↦ᵣ WCap p_pc b_pc e_pc (a_spinlock ^+ 3)%a )%I with "[HPC]"
-        as "HPC".
-      { inversion HPC_exec ; auto ; subst ; iFrame. }
-      iApply ("IH" with "[$Hr0] [$Hr3] [$Hb_lock]
-                         [$Hφ] [$Hr1] [$HPC] [$Hr2]").
-Qed.
-
-
-
-  Definition malloc_pre_spin (offset : Z) :=
+  (* TODO we actually NEED to store the capability pointing to the lock,
+          because we only have the RX permission, not RWX. *)
+  (* offset_lock = last address of the free memory *)
+  Definition malloc_pre_spin (offset_lock : Z) :=
     encodeInstrsW [
         (* bm: *)
      Lt r_t3 0 r_t1; (* ;; check that size > 0 *)
@@ -111,14 +47,14 @@ Qed.
      Jnz r_t2 r_t3;  (* ;; fail if not         *)
      Fail;
         (* xm: *)
-     Mov r_t2 PC;
-        (* Spinlock: wait until the malloc is available *)
-        (* rt5, rt6, rt7, rt8 are used for the spinlock *)
      Mov r_t5 PC;
-     Lea r_t5 (offset + 1)%Z].
+     Lea r_t5 (offset_lock - 5)%Z;
+     Load r_t5 r_t5
+      ].
 
   Definition malloc_post_spin (offset : Z) :=
     encodeInstrsW [
+     Mov r_t2 PC;
      Lea r_t2 offset;
      (* ;; r2 = (RWX, bm, em, bmid) *)
      Load r_t2 r_t2;  (* ;; r2 = (RWX, bmid, em, a)  *)
@@ -137,7 +73,7 @@ Qed.
      Lea r_t3 r_t1;   (* ;; r3 = (RWX, bmid, em, bmid)       *)
      Store r_t3 r_t2; (* ;; bmid <- (RWX, bmid, em, a+size)  *)
      Mov r_t1 r_t4;   (* ;; r3 = (RWX, a, a+size, a)         *)
-     Store r_t8 0;    (* Release the lock - we don't need CAS *)
+     Store r_t5 0;    (* Release the lock - we don't need CAS *)
      Mov r_t2 0%Z;    (* Clear the registers *)
      Mov r_t3 0%Z;
      Mov r_t4 0%Z;
@@ -155,8 +91,8 @@ Qed.
       ].
 
 
-  Definition malloc_subroutine_instrs' (offset: Z) :=
-     malloc_pre_spin offset
+  Definition malloc_subroutine_instrs' (offset offset_lock: Z) :=
+     malloc_pre_spin offset_lock
        ++ spinlock_instrs' r_t5 r_t6 r_t7 r_t8
        ++ malloc_post_spin offset.
 
@@ -170,27 +106,105 @@ Qed.
     Eval cbv in (length (spinlock_instrs' PC PC PC PC)).
 
   Definition malloc_subroutine_instrs_length : Z :=
-    Eval cbv in (length (malloc_subroutine_instrs' 0%Z)).
+    Eval cbv in (length (malloc_subroutine_instrs' 0%Z 0%Z)).
 
-  Definition malloc_subroutine_instrs :=
-    malloc_subroutine_instrs' (malloc_subroutine_instrs_length - 5).
+  Definition malloc_subroutine_instrs (offset_lock : Z) :=
+    malloc_subroutine_instrs'
+      (malloc_subroutine_instrs_length - (5+spinlock_length))
+      offset_lock.
 
-  Definition malloc_inv (b e : Addr) : iProp Σ :=
-    (codefrag b malloc_subroutine_instrs
-     ∗ ∃ b_m a_m,
-        ⌜(b + malloc_subroutine_instrs_length)%a = Some b_m⌝
-     ∗ b_m ↦ₐ (WCap RWX b_m e a_m)
-     ∗ ((b_m ^+1)%a ↦ₐ (WInt 0) ∨ (b_m ^+1)%a ↦ₐ (WInt 1))
-     ∗ [[a_m, e]] ↦ₐ [[ region_addrs_zeroes a_m e ]]
-     ∗ ⌜(b_m < a_m)%a ∧ (a_m <= e)%a⌝)%I.
+  Definition malloc_inv (b e : Addr) γ : iProp Σ :=
+    (codefrag b (malloc_subroutine_instrs e)
+     ∗ e ↦ₐ WCap RWX b (e^+2)%a (e^+1)%a
+     ∗ is_lock γ (e ^+1)%a
+         (  ∃ b_m a_m,
+             ⌜(b + malloc_subroutine_instrs_length)%a = Some b_m⌝
+             ∗ b_m ↦ₐ (WCap RWX b_m e a_m)
+             ∗ [[a_m, e]] ↦ₐ [[ region_addrs_zeroes a_m e ]]
+             ∗ ⌜(b_m < a_m)%a ∧ (a_m <= e)%a⌝)%I).
 
+
+  Lemma malloc_prelock_spec
+    (i : CoreN)
+    (wsize: Word)
+    (b e : Addr)
+    w2 w3 w5
+    N E
+    (φ : language.val cap_lang → iProp Σ) :
+
+    let e' := (e^+2)%a in
+    SubBounds b e' b (b ^+ malloc_subroutine_instrs_length)%a ->
+    ↑N ⊆ E →
+    (    inv N (codefrag b (malloc_pre_spin e)
+                ∗ e ↦ₐ WCap RWX b e' (e^+1)%a)
+         ∗ (i, PC) ↦ᵣ WCap RX b e' b
+         ∗ (i, r_t1) ↦ᵣ wsize
+         ∗ (i, r_t2) ↦ᵣ w2
+         ∗ (i, r_t3) ↦ᵣ w3
+         ∗ (i, r_t5) ↦ᵣ w5
+         ∗ ▷ (   (i, PC) ↦ᵣ WCap RX b e' (b ^+ malloc_pre_spin_length)%a
+                 ∗ (i, r_t1) ↦ᵣ wsize
+                 ∗ (i, r_t2) ↦ᵣ WCap RX b e' (b ^+ 5)%a
+                 ∗ (i, r_t3) ↦ᵣ WInt 1%nat
+                 ∗ (i, r_t5) ↦ᵣ WCap RWX b e' (e ^+1)%a
+                 ∗ ⌜ exists size:Z, (0 < size)%Z /\ wsize = WInt size ⌝
+                 -∗ WP (i, Seq (Instr Executable)) @ E {{ φ }}%I))
+    ⊢ WP (i, Seq (Instr Executable)) @ E {{ λ v, φ v ∨ ⌜v = (i, FailedV)⌝ }}%I.
+  Proof.
+    intro e'.
+    iIntros (Hbounds HN) "(#Hfinv & HPC & Hr1 & Hr2 & Hr3 & Hr5 & Hφ)".
+    iDestruct (inv_split_l with "Hfinv") as "Hinv".
+    destruct (wsize) as [size|].
+
+    2: { iInstr_inv "Hinv". wp_end. eauto. }
+    do 3 iInstr_inv "Hinv".
+
+    (* we need to destruct on the cases for the size *)
+    destruct (decide (0 < size)%Z) as [Hsize | Hsize].
+    2: { (* the program will not jump, and go to the fail instruction *)
+      rewrite (_: Z.b2z (0%nat <? size)%Z = 0); cycle 1.
+      { apply Z.ltb_nlt in Hsize. rewrite Hsize //. }
+      iInstr_inv "Hinv". iInstr_inv "Hinv". wp_end. eauto. }
+
+    rewrite (_: Z.b2z (0%nat <? size)%Z = 1); cycle 1.
+    { rewrite (_: (0%nat <? size)%Z = true ); auto. by apply Z.ltb_lt. }
+
+
+    do 3 iInstr_inv "Hinv".
+    { transitivity (Some e). admit. done. }
+
+    wp_instr
+    ; iInv "Hfinv" as ">[Hprog Hcaplock]" "Hcls"
+    ; codefrag_facts "Hprog" (* TODO fix this, because it duplicates the hypothesis *).
+    iInstr_lookup "Hprog" as "Hi" "Hcont".
+    iApply ( wp_load_success_same_notinstr with "[$HPC $Hi $Hr5 $Hcaplock]").
+    { exact (WInt 0). } (* TODO : why do I have to provide a word ? *)
+    { rewrite decode_encode_instrW_inv ; auto. }
+    { apply isCorrectPC_intro; [admit| auto]. }
+    { auto. }
+    { admit. }
+    { transitivity (Some (b ^+8)%a) ; solve_addr ; done. }
+    iNext ; iIntros "(HPC & Hr5 & Hi & Hcaplock)".
+    iDestruct ("Hcont" with "Hi") as "Hprog".
+    iMod ("Hcls" with "[$Hprog $Hcaplock]") as "_".
+    simpl ; iModIntro ; wp_pure.
+
+    iApply (wp_wand with "[-]").
+    { iApply "Hφ".
+      rewrite /malloc_pre_spin_length.
+      iFrame.
+      iPureIntro. eexists. split ; eauto. }
+    iIntros (?) "?" ; iFrame.
+  Admitted.
+
+  
   Lemma simple_malloc_subroutine_spec
     (i : CoreN)
     (wsize: Word)
     (cont: Word)
     (b e : Addr)
     (rmap : (gmap (CoreN * RegName) Word))
-    N E
+    N E γ
     (φ : language.val cap_lang → iProp Σ) :
 
     dom (gset (CoreN*RegName)) rmap =
@@ -198,14 +212,18 @@ Qed.
 
     (exists b_m, (b + malloc_subroutine_instrs_length)%a = Some b_m /\ (b_m < e)%a) ->
     ↑N ⊆ E →
-    (  inv N (malloc_inv b e)
+    (  inv N (malloc_inv b e γ)
      ∗ ([∗ map] r↦w ∈ rmap, r ↦ᵣ w)
      ∗ (i, r_t0) ↦ᵣ cont
-     ∗ (i, PC) ↦ᵣ WCap RX b e b
+     ∗ (i, PC) ↦ᵣ WCap RX b (e ^+2)%a b
      ∗ (i, r_t1) ↦ᵣ wsize
        ∗ ▷ (([∗ map] r↦w ∈ <[(i, r_t2) := WInt 0%Z]>
                (<[(i, r_t3) := WInt 0%Z]>
-                  (<[(i, r_t4) := WInt 0%Z]> rmap)), r ↦ᵣ w)
+                  (<[(i, r_t4) := WInt 0%Z]>
+                     (<[(i, r_t5) := WInt 0%Z]>
+                        (<[(i, r_t6) := WInt 0%Z]>
+                           (<[(i, r_t7) := WInt 0%Z]>
+                              (<[(i, r_t8) := WInt 0%Z]> rmap)))))), r ↦ᵣ w)
             ∗ (i, r_t0) ↦ᵣ cont
             ∗ (i, PC) ↦ᵣ updatePcPerm cont
             ∗ (∃ (ba ea : Addr) size,
@@ -219,7 +237,7 @@ Qed.
     iIntros (Hrmap_dom Hbm HN) "(#Hinv & Hrmap & Hr0 & HPC & Hr1 & Hφ)".
     destruct Hbm as ( bm & Hbm & Hbme ).
     unfold malloc_subroutine_instrs_length in Hbm.
-    assert (Hbounds: SubBounds b e b (b ^+ length malloc_subroutine_instrs)%a) by solve_addr.
+    assert (Hbounds: SubBounds b (e ^+ 2)%a b (b ^+ (length (malloc_subroutine_instrs e)))%a) by solve_addr.
     rewrite /malloc_inv.
 
     (* Get some registers *)
@@ -269,22 +287,31 @@ Qed.
 
 
     (* Split the invariant into more fine-grained invariant *)
-    iDestruct (inv_split_l with "Hinv") as "Hinv_code".
+    iDestruct (inv_split with "Hinv") as "[Hinv_code Hinv_lock]".
     rewrite {2}/codefrag.
     rewrite {2}/malloc_subroutine_instrs /malloc_subroutine_instrs'.
     rewrite (region_mapsto_split _ _ (b ^+ malloc_pre_spin_length)%a).
     2:{ cbn; rewrite /malloc_pre_spin_length; solve_addr. }
-    2:{ cbn; rewrite /malloc_pre_spin_length. admit. }
+    2:{ cbn; rewrite /malloc_pre_spin_length.
+        assert (H0 : (b+8)%f = Some (b ^+8)%a) by solve_addr.
+        apply (finz_incr_iff_dist b (b ^+8)%a 8%nat) in H0.
+        destruct H0 as [_ ?].
+        symmetry. apply H0. }
     rewrite (region_mapsto_split (b ^+ malloc_pre_spin_length)%a _
                ((b ^+ malloc_pre_spin_length ^+ spinlock_length)%a)).
     2:{ rewrite /malloc_pre_spin_length /spinlock_length; solve_addr. }
-    2:{ cbn. admit. }
+    2:{ cbn; rewrite /malloc_pre_spin_length /spinlock_length.
+        set (b' := (b ^+ 8)%a).
+        assert (H0 : ((b ^+ 8)%a+6)%f = Some ((b ^+ 8)%a ^+6)%a) by solve_addr.
+        apply (finz_incr_iff_dist b' (b' ^+6)%a 6%nat) in H0.
+        destruct H0 as [_ ?].
+        symmetry. apply H0. }
     iDestruct (inv_split with "Hinv_code") as "[Hinv_code_pre H']".
     iDestruct (inv_split with "H'") as "[Hinv_code_spin Hinv_code_post]".
     iClear "Hinv_code"; iClear "H'".
     rewrite /length /=.
 
-    iAssert ( inv N (codefrag b (malloc_pre_spin (malloc_subroutine_instrs_length - 5))))
+    iAssert ( inv N (codefrag b (malloc_pre_spin e)))
               as "Hinv_pre"  ; first iFrame "#".
     iClear "Hinv_code_pre".
 
@@ -294,55 +321,120 @@ Qed.
     iClear "Hinv_code_spin".
 
     iAssert ( inv N (codefrag ((b ^+ malloc_pre_spin_length) ^+ spinlock_length)%a
-                       (malloc_post_spin (malloc_subroutine_instrs_length - 5))))
+                       (malloc_post_spin (malloc_subroutine_instrs_length - (5 + spinlock_length)))))
               as "Hinv_post"
     ; first ( iFrame "#"
          ; rewrite /codefrag
          ; simpl ; rewrite /malloc_pre_spin_length /malloc_pre_post_length /spinlock_length
-         ; replace ((((b ^+ 8) ^+ 6) ^+ 25%nat)%a) with (b ^+ 39%nat)%a by solve_addr
+         ; replace ((((b ^+ 8) ^+ 6) ^+ 26%nat)%a) with (b ^+ 40%nat)%a by solve_addr
          ; iFrame "#").
     iClear "Hinv_code_post".
 
-    (* Lt *)
-    wp_instr.
-    iInv "Hinv_pre" as ">Hprog" "Hcls".
-    codefrag_facts "Hprog".
+    (** ====== Pre lock ====== *)
 
-    destruct (wsize) as [size|].
-    2: {
-      iInstr_lookup "Hprog" as "Hi" "Hcont".
-      iApply ( wp_add_sub_lt_fail_z_r with "[ $HPC $Hr3 $Hr1 $Hi ]") ; eauto.
-      { cbn; rewrite decode_encode_instr_inv; auto. }
-      { apply isCorrectPC_intro ; [solve_addr| auto]. }
-      iModIntro. iIntros "Hb".
-      iDestruct ("Hcont" with "Hb") as "Hprog".
-      cbn.
-      iMod ("Hcls" with "Hprog") as "_".
-      iModIntro. wp_pure; wp_end; cbn. eauto. }
+    iApply (wp_wand_l _ _ _ (λ v, ((φ v ∨ ⌜v = (i, FailedV)⌝) ∨ ⌜v = (i, FailedV)⌝)))%I. iSplitR.
+    { iIntros (v) "[H|H] /=";auto. }
+    iApply (malloc_prelock_spec _ _ _ _ _ _ _ _ _ (fun v => (φ v ∨ ⌜v = (i, FailedV)⌝)%I)
+             with "[-$HPC $Hr1 $Hr2 $Hr3 $Hr5 Hinv_pre]") ;eauto.
+    iSplitR.
+   { iClear "Hinv_lock"
+      ; iClear "Hinv_pre"
+      ; iClear "Hinv_spin"
+      ; iClear "Hinv_post".
 
-    iInstr_lookup "Hprog" as "Hi" "Hcont".
-    iApply ( wp_add_sub_lt_success_z_r with "[ $HPC $Hr1 $Hr3 $Hi ]") ; eauto.
-    { cbn; rewrite decode_encode_instr_inv; eauto. }
-    { transitivity (Some (b ^+ 1)%a); solve_addr; done. }
-    { apply isCorrectPC_intro ; [solve_addr| auto]. }
-    iNext. iIntros "(HPC & Hi & Hr1 & Hr3)".
-    rewrite decode_encode_instrW_inv.
-    rewrite /denote.
-    iDestruct ("Hcont" with "Hi") as "Hprog".
-    iMod ("Hcls" with "Hprog") as "_".
-    simpl ; iModIntro ; wp_pure.
+    (* iDestruct (inv_split with "Hinv") as "[Hinv_code Hinv_lock]". *)
+    rewrite {1}/codefrag.
+    rewrite {1}/malloc_subroutine_instrs /malloc_subroutine_instrs'.
+    rewrite (region_mapsto_split _ _ (b ^+ malloc_pre_spin_length)%a).
+    2:{ cbn; rewrite /malloc_pre_spin_length; solve_addr. }
+    2:{ cbn; rewrite /malloc_pre_spin_length.
+        assert (H' : (b+8)%f = Some (b ^+8)%a) by solve_addr.
+        apply (finz_incr_iff_dist b (b ^+8)%a 8%nat) in H'.
+        destruct H' as [_ H'].
+        symmetry; apply H'. }
+    rewrite (region_mapsto_split (b ^+ malloc_pre_spin_length)%a _
+               ((b ^+ malloc_pre_spin_length ^+ spinlock_length)%a)).
+    2:{ rewrite /malloc_pre_spin_length /spinlock_length; solve_addr. }
+    2:{ cbn; rewrite /malloc_pre_spin_length /spinlock_length.
+        set (b' := (b ^+ 8)%a).
+        assert (H' : ((b ^+ 8)%a+6)%f = Some ((b ^+ 8)%a ^+6)%a) by solve_addr.
+        apply (finz_incr_iff_dist b' (b' ^+6)%a 6%nat) in H'.
+        destruct H' as [_ H'].
+        symmetry; apply H'. }
+    match goal with
+    | h: _ |- context [ is_lock ?g ?b ?P] => set (L := is_lock g b P)
+    end.
+    match goal with
+    | h: _ |- context [ region_mapsto ?b ?e ?l ] => set (P1 := region_mapsto b e l)
+    end.
+    match goal with
+    | h: _ |- context [ region_mapsto ?b ?e ?l ] => set (P2 := region_mapsto b e l)
+    end.
+    match goal with
+    | h: _ |- context [ region_mapsto ?b ?e ?l ] => set (P3 := region_mapsto b e l)
+    end.
+    match goal with
+    | h: _ |- context [ mapsto ?e ?d ?v ] => set (IE := mapsto e d v)
+    end.
+    simpl.
+    iAssert ( inv N ( (P1 ∗ IE) ∗ ( P2 ∗ P3 ) ∗ L ) ) as "Hinv1".
+    iApply (inv_iff with "[$Hinv]")
+     ; first (do 2 iModIntro ; iSplit ;
+              [iIntros "((?&?&?) & ? & ?)" | iIntros "((? & ?) & (?&?) & ?)" ]
+               ; iFrame).
+    iDestruct (inv_split_l with "Hinv1") as "Hinv2".
+    iClear "Hinv" ; iClear "Hinv1" ; clear -P1.
+    assert (P1 =  codefrag b (malloc_pre_spin e)).
+    { subst P1. rewrite /codefrag /malloc_pre_spin /malloc_pre_spin_length.
+      by cbn. }
+    auto.
+    }
+    iNext ; iIntros "(HPC & Hr1 & Hr2 & Hr3 & Hr5 & %Hsize)".
+    destruct Hsize as (size & ? & ->).
+
+    (** ====== Spinlock ====== *)
+    iApply (spinlock_spec i _ _ _ _ r_t5 r_t6 r_t7 r_t8 with
+             "[-$HPC $Hr5 $Hr6 $Hr7 $Hr8]")
+    ;[ apply ExecPCPerm_RX
+       |.. ].
+    { rewrite /malloc_pre_spin_length ; solve_addr. }
+    { auto. }
+    { admit. }
+    { eauto. }
+    iSplitR.
+    { iAssert ( inv N (codefrag (b ^+ 8)%a (spinlock_instrs' r_t5 r_t6 r_t7 r_t8)
+                       ∗ is_lock γ (e ^+1)%a (∃ b_m a_m : Addr,
+                               ⌜(b + malloc_subroutine_instrs_length)%a = Some b_m⌝
+                                                                          ∗ b_m ↦ₐ WCap RWX b_m e a_m
+                                                                          ∗
+                                                                            [[a_m,e]]↦ₐ[[region_addrs_zeroes a_m e]] ∗ ⌜(b_m < a_m)%a ∧ (a_m <= e)%a⌝)))%I
+                as "Hinv_spinlock" .
+      admit.
+      iFrame "Hinv_spinlock". }
+    iNext ; iIntros "(HPC & Hr5 & Hr6 & Hr7 & Hr8 & Hbm & Hlocked)".
+
+    (** ====== Post-Lock ======*)
+    iDestruct "Hbm"
+      as (b_m a_m) "(%Hbm_bounds & Hb_m & Hfree_reg & %Ham_bounds)".
+    rewrite /length /=.
+    replace ( ((b ^+ malloc_pre_spin_length) ^+ 6%nat)%a )
+      with (b ^+ 14)%a
+           by (rewrite /malloc_pre_spin_length ; solve_addr).
+    replace ( ((b ^+ malloc_pre_spin_length) ^+ spinlock_length)%a )
+      with (b ^+ 14)%a
+           by (rewrite /malloc_pre_spin_length /spinlock_length ; solve_addr).
+
 
     (* Mov *)
     (* Open the invariant *)
     wp_instr
-    ; iInv "Hinv_pre" as ">Hprog" "Hcls"
-    ; codefrag_facts "Hprog".
+    ; iInv "Hinv_post" as ">Hprog" "Hcls"
     (* Apply the invariant *)
-    iInstr_lookup "Hprog" as "Hi" "Hcont"
-    ; iApply ( wp_move_success_reg_fromPC with "[ $HPC Hr2 $Hi ]") ; eauto.
+    ; iInstr_lookup "Hprog" as "Hi" "Hcont".
+    iApply ( wp_move_success_reg_fromPC with "[ $HPC $Hr2 $Hi ]") ; eauto.
     { cbn ;rewrite decode_encode_instr_inv; eauto. }
     { apply isCorrectPC_intro ; [solve_addr| auto]. }
-    { transitivity (Some (b ^+ 2)%a); solve_addr; done. }
+    { transitivity (Some ((b ^+ 14) ^+1)%a); solve_addr; done. }
     iNext; iIntros "(HPC & Hi & Hr2)".
     (* Close the invariant *)
     iDestruct ("Hcont" with "Hi") as "Hprog".
@@ -352,142 +444,711 @@ Qed.
     (* Lea *)
     (* Open the invariant *)
     wp_instr
-    ; iInv "Hinv_pre" as ">Hprog" "Hcls"
-    ; codefrag_facts "Hprog".
+    ; iInv "Hinv_post" as ">Hprog" "Hcls"
     (* Apply the invariant *)
-    iInstr_lookup "Hprog" as "Hi" "Hcont"
-    ; iApply ( wp_lea_success_z with "[ $HPC $Hr2 $Hi ]") ; eauto.
+    ; iInstr_lookup "Hprog" as "Hi" "Hcont".
+    iApply ( wp_lea_success_z with "[ $HPC $Hr2 $Hi ]") ; eauto.
     { cbn ;rewrite decode_encode_instr_inv; eauto. }
     { apply isCorrectPC_intro ; [solve_addr| auto]. }
-    { transitivity (Some (b ^+ 3)%a); solve_addr; done. }
-    { transitivity (Some (b ^+ 5)%a); solve_addr; done. }
+    { transitivity (Some ((b ^+ 14) ^+2)%a); solve_addr; done. }
+    { transitivity (Some (b ^+ 39)%a)
+      ; rewrite /spinlock_length /malloc_subroutine_instrs_length.
+      admit. done. } (* TODO correct the offset *)
+      (* ; solve_addr; done. } *)
     iNext; iIntros "(HPC & Hi & Hr2)".
     (* Close the invariant *)
     iDestruct ("Hcont" with "Hi") as "Hprog".
     iMod ("Hcls" with "Hprog") as "_".
     simpl ; iModIntro ; wp_pure.
 
-    (* we need to destruct on the cases for the size *)
-    destruct (decide (0 < size)%Z) as [Hsize | Hsize].
-    2: { (* the program will not jump, and go to the fail instruction *)
-      rewrite (_: Z.b2z (0%nat <? size)%Z = 0); cycle 1.
-      { apply Z.ltb_nlt in Hsize. rewrite Hsize //. }
-      wp_instr
-      ; iInv "Hinv_pre" as ">Hprog" "Hcls"
-      ; codefrag_facts "Hprog".
-      (* Apply the invariant *)
-      iInstr_lookup "Hprog" as "Hi" "Hcont"
-      ; iApply ( wp_jnz_success_next with "[ $HPC $Hr2 Hr3 $Hi ]") ; eauto.
-      { cbn ;rewrite decode_encode_instr_inv; eauto. }
-      { apply isCorrectPC_intro ; [solve_addr| auto]. }
-      { transitivity (Some (b ^+ 4)%a); solve_addr; done. }
-      iNext; iIntros "(HPC & Hi & Hr2 & Hr3)".
-      (* Close the invariant *)
-      iDestruct ("Hcont" with "Hi") as "Hprog".
-      iMod ("Hcls" with "Hprog") as "_".
-      simpl ; iModIntro ; wp_pure.
 
-      wp_instr
-      ; iInv "Hinv_pre" as ">Hprog" "Hcls"
-      ; codefrag_facts "Hprog".
-      iInstr_lookup "Hprog" as "Hi" "Hcont"
-      ; iApply ( wp_fail with "[ $HPC $Hi ]") ; eauto.
-      { cbn ;rewrite decode_encode_instr_inv; eauto. }
-      { apply isCorrectPC_intro ; [solve_addr| auto]. }
-      iNext; iIntros "(HPC & Hi)".
-      (* Close the invariant *)
-      iDestruct ("Hcont" with "Hi") as "Hprog".
-      iMod ("Hcls" with "Hprog") as "_".
-      simpl ; iModIntro ; wp_pure.
-      wp_end ; eauto.
-      }
-
-
-    rewrite (_: Z.b2z (0%nat <? size)%Z = 1); cycle 1.
-    { rewrite (_: (0%nat <? size)%Z = true ); auto. by apply Z.ltb_lt. }
-
-    (* Lea *)
+    (* Load *)
     (* Open the invariant *)
+    replace (b ^+ 39)%a with b_m by admit.
+    (* by (rewrite /malloc_subroutine_instrs_length *)
+    (*                              in Hbm_bounds ; solve_addr). *)
     wp_instr
-    ; iInv "Hinv_pre" as ">Hprog" "Hcls"
-    ; codefrag_facts "Hprog".
+    ; iInv "Hinv_post" as ">Hprog" "Hcls"
     (* Apply the invariant *)
-    iInstr_lookup "Hprog" as "Hi" "Hcont"
-    ; iApply ( wp_jnz_success_jmp with "[ $HPC $Hr2 $Hr3 $Hi ]") ; eauto.
+    ; iInstr_lookup "Hprog" as "Hi" "Hcont".
+    iApply ( wp_load_success_same_notinstr with "[ $HPC $Hr2 $Hi $Hb_m]") ; eauto.
     { cbn ;rewrite decode_encode_instr_inv; eauto. }
     { apply isCorrectPC_intro ; [solve_addr| auto]. }
+    { rewrite /malloc_subroutine_instrs_length in Hbm_bounds
+      ; solve_addr. }
+    { transitivity (Some ((b ^+ 14) ^+3)%a); solve_addr; done. }
+    iNext ; iIntros "(HPC & Hr2 & Hi & Hbm)".
+    (* Close the invariant *)
+    iDestruct ("Hcont" with "Hi") as "Hprog".
+    iMod ("Hcls" with "Hprog") as "_".
+    simpl ; iModIntro ; wp_pure.
+
+    (* GetA *)
+    (* Open the invariant *)
+    wp_instr
+    ; iInv "Hinv_post" as ">Hprog" "Hcls"
+    (* Apply the invariant *)
+    ; iInstr_lookup "Hprog" as "Hi" "Hcont".
+    iApply ( wp_Get_success with "[ $HPC $Hr3 $Hr2 $Hi ]") ; eauto.
+    { cbn ;rewrite decode_encode_instr_inv; eauto. }
+    { apply isCorrectPC_intro ; [solve_addr| auto]. }
+    { transitivity (Some ((b ^+ 14) ^+4)%a); solve_addr; done. }
     iNext; iIntros "(HPC & Hi & Hr2 & Hr3)".
     (* Close the invariant *)
     iDestruct ("Hcont" with "Hi") as "Hprog".
     iMod ("Hcls" with "Hprog") as "_".
     simpl ; iModIntro ; wp_pure.
+    rewrite decode_encode_instr_inv /rules_Get.denote.
+
+
+    (* Lea might fail *)
+
+    (* Lea *)
+    (* Open the invariant *)
+    wp_instr
+    ; iInv "Hinv_post" as ">Hprog" "Hcls"
+    (* Apply the invariant *)
+    ; iInstr_lookup "Hprog" as "Hi" "Hcont".
+
+    destruct (a_m + size)%a as [a_m'|] eqn:Ha_m'; cycle 1.
+    { (* Failure case: no registered rule for that yet; do it the manual way *)
+      (* TODO: cf malloc, do not use rmap, but an empty map *)
+      iAssert ([∗ map] k↦x ∈ (∅:gmap (CoreN * RegName) Word), k ↦ᵣ x)%I as "-#Hregs".
+        by rewrite big_sepM_empty.
+
+      iDestruct (big_sepM_insert with "[$Hregs $Hr2]") as "Hregs".
+      by rewrite lookup_empty.
+      iDestruct (big_sepM_insert with "[$Hregs $Hr1]") as "Hregs".
+      rewrite !lookup_insert_ne
+      ; first by rewrite lookup_empty.
+      all: try (match goal with
+                | h:_ |- _ ≠ _ => simplify_pair_eq
+                end).
+      iDestruct (big_sepM_insert with "[$Hregs $HPC]") as "Hregs".
+      rewrite !lookup_insert_ne
+      ; first by rewrite lookup_empty.
+      all: try (match goal with
+                | h:_ |- _ ≠ _ => simplify_pair_eq
+                end).
+
+
+      iApply (wp_lea _ i RX b (e ^+2)%a ((b ^+ 14) ^+ 4)%a
+               with "[$Hregs $Hi]").
+      { rewrite decode_encode_instrW_inv; done. }
+      { admit. }
+      { apply lookup_insert. }
+      { rewrite /regs_of_core !dom_insert_L dom_empty_L. set_solver-. }
+      iNext. iIntros (regs' retv) "(Hspec & Hi & ?)".
+      iDestruct "Hspec" as %Hspec.
+
+      iDestruct ("Hcont" with "Hi") as "Hprog".
+      iMod ("Hcls" with "Hprog") as "_".
+
+      destruct Hspec as [| Hfail].
+      { exfalso.
+        clear - H4 Ha_m' H3 H1.
+        simplify_map_eq by simplify_pair_eq. }
+      { cbn.
+        iApply wp_pure_step_later; auto.
+        do 2 iModIntro.
+        iApply wp_value.
+        auto. } }
+
+
+
+    iApply ( wp_lea_success_reg with "[ $HPC $Hr2 $Hr1 $Hi ]") ; eauto.
+    { cbn ;rewrite decode_encode_instr_inv; eauto. }
+    { apply isCorrectPC_intro ; [solve_addr| auto]. }
+    { transitivity (Some ((b ^+ 14) ^+5)%a); solve_addr; done. }
+    iNext; iIntros "(HPC & Hi & Hr1 & Hr2)".
+    (* Close the invariant *)
+    iDestruct ("Hcont" with "Hi") as "Hprog".
+    iMod ("Hcls" with "Hprog") as "_".
+    simpl ; iModIntro ; wp_pure.
+
+    (* GetA *)
+    (* Open the invariant *)
+    wp_instr
+    ; iInv "Hinv_post" as ">Hprog" "Hcls"
+    (* Apply the invariant *)
+    ; iInstr_lookup "Hprog" as "Hi" "Hcont".
+    iApply ( wp_Get_success with "[ $HPC $Hr1 $Hr2 $Hi ]") ; eauto.
+    { cbn ;rewrite decode_encode_instr_inv; eauto. }
+    { apply isCorrectPC_intro ; [solve_addr| auto]. }
+    { transitivity (Some ((b ^+ 14) ^+6)%a); solve_addr; done. }
+    iNext; iIntros "(HPC & Hi & Hr2 & Hr1)".
+    (* Close the invariant *)
+    iDestruct ("Hcont" with "Hi") as "Hprog".
+    iMod ("Hcls" with "Hprog") as "_".
+    simpl ; iModIntro ; wp_pure.
+    rewrite decode_encode_instr_inv /rules_Get.denote.
 
     (* Mov *)
     (* Open the invariant *)
     wp_instr
-    ; iInv "Hinv_pre" as ">Hprog" "Hcls"
-    ; codefrag_facts "Hprog".
+    ; iInv "Hinv_post" as ">Hprog" "Hcls"
     (* Apply the invariant *)
-    iInstr_lookup "Hprog" as "Hi" "Hcont"
-    ; iApply ( wp_move_success_reg_fromPC with "[ $HPC $Hr2 $Hi ]") ; eauto.
+    ; iInstr_lookup "Hprog" as "Hi" "Hcont".
+    iApply ( wp_move_success_reg with "[ $HPC $Hr4 $Hr2 $Hi ]") ; eauto.
     { cbn ;rewrite decode_encode_instr_inv; eauto. }
     { apply isCorrectPC_intro ; [solve_addr| auto]. }
-    { transitivity (Some (b ^+ 6)%a); solve_addr; done. }
+    { transitivity (Some ((b ^+ 14) ^+7)%a); solve_addr; done. }
+    iNext; iIntros "(HPC & Hi & Hr4 & Hr2)".
+    (* Close the invariant *)
+    iDestruct ("Hcont" with "Hi") as "Hprog".
+    iMod ("Hcls" with "Hprog") as "_".
+    simpl ; iModIntro ; wp_pure.
+    (* might fail *)
+    (* subseg *)
+    (* Open the invariant *)
+    wp_instr
+    ; iInv "Hinv_post" as ">Hprog" "Hcls"
+    (* Apply the invariant *)
+    ; iInstr_lookup "Hprog" as "Hi" "Hcont".
+
+    destruct (isWithin a_m a_m' b_m e) eqn:Ha_m'_within; cycle 1.
+    { (* Failure case: manual mode. *)
+      iAssert ([∗ map] k↦x ∈ (∅:gmap (CoreN * RegName) Word), k ↦ᵣ x)%I as "-#Hregs".
+        by rewrite big_sepM_empty.
+
+      iDestruct (big_sepM_insert with "[$Hregs $Hr4]") as "Hregs".
+      by rewrite lookup_empty.
+      iDestruct (big_sepM_insert with "[$Hregs $Hr3]") as "Hregs".
+      rewrite !lookup_insert_ne
+      ; first by rewrite lookup_empty.
+      all: try (match goal with
+                | h:_ |- _ ≠ _ => simplify_pair_eq
+                end).
+      iDestruct (big_sepM_insert with "[$Hregs $Hr1]") as "Hregs".
+      rewrite !lookup_insert_ne
+      ; first by rewrite lookup_empty.
+      all: try (match goal with
+                | h:_ |- _ ≠ _ => simplify_pair_eq
+                end).
+      iDestruct (big_sepM_insert with "[$Hregs $HPC]") as "Hregs".
+      rewrite !lookup_insert_ne
+      ; first by rewrite lookup_empty.
+      all: try (match goal with
+                | h:_ |- _ ≠ _ => simplify_pair_eq
+                end).
+
+      iApply (wp_Subseg with "[$Hregs $Hi]").
+      { rewrite decode_encode_instrW_inv; done. }
+      { admit. }
+      { apply lookup_insert. }
+      { rewrite /regs_of_core !dom_insert_L dom_empty_L. set_solver-. }
+      iNext. iIntros (regs' retv) "(Hspec & Hi & ?)".
+
+      iDestruct ("Hcont" with "Hi") as "Hprog".
+      iMod ("Hcls" with "Hprog") as "_".
+
+      iDestruct "Hspec" as %Hspec.
+      destruct Hspec as [| Hfail].
+      { exfalso. unfold addr_of_argument in *.
+        clear -H1 H3 H4 H5 Ha_m'_within.
+        simplify_map_eq by simplify_pair_eq.
+        repeat match goal with H:_ |- _ => apply finz_of_z_eq_inv in H end; subst.
+        congruence. }
+      { cbn. iModIntro. wp_pure. wp_end. auto. } }
+
+
+    
+    iApply ( wp_subseg_success with "[ $HPC $Hr4 $Hr3 $Hr1 $Hi ]") ; eauto.
+    { cbn ;rewrite decode_encode_instr_inv; eauto. }
+    { apply isCorrectPC_intro ; [solve_addr| auto]. }
+    { transitivity (Some a_m); solve_addr; done. }
+    { transitivity (Some (a_m ^+ size)%a); solve_addr; done. }
+    { transitivity (Some ((b ^+ 14) ^+8)%a); solve_addr; done. }
+    iNext; iIntros "(HPC & Hi & Hr3 & Hr1 & Hr4)".
+    (* Close the invariant *)
+    iDestruct ("Hcont" with "Hi") as "Hprog".
+    iMod ("Hcls" with "Hprog") as "_".
+    simpl ; iModIntro ; wp_pure.
+
+
+    (* sub *)
+    (* Open the invariant *)
+    wp_instr
+    ; iInv "Hinv_post" as ">Hprog" "Hcls"
+    (* Apply the invariant *)
+    ; iInstr_lookup "Hprog" as "Hi" "Hcont".
+    iApply ( wp_add_sub_lt_success_dst_r with "[ $HPC $Hr1 $Hr3 $Hi ]") ; eauto.
+    { rewrite decode_encode_instrW_inv ;cbn ; auto. }
+    { transitivity (Some ((b ^+ 14) ^+9)%a); solve_addr; done. }
+    { apply isCorrectPC_intro ; [solve_addr| auto]. }
+    iNext; iIntros "(HPC & Hi & Hr1 & Hr3)".
+    (* Close the invariant *)
+    iDestruct ("Hcont" with "Hi") as "Hprog".
+    iMod ("Hcls" with "Hprog") as "_".
+    simpl ; iModIntro ; wp_pure.
+    rewrite decode_encode_instr_inv /denote /=.
+    (* replace (a_m - (a_m ^+ size)%a)%Z with (-size)%Z by admit. *)
+
+    (* Lea *)
+    (* Open the invariant *)
+    wp_instr
+    ; iInv "Hinv_post" as ">Hprog" "Hcls"
+    (* Apply the invariant *)
+    ; iInstr_lookup "Hprog" as "Hi" "Hcont".
+    iApply ( wp_lea_success_reg with "[ $HPC $Hr4 $Hr3 $Hi ]") ; eauto.
+    { cbn ;rewrite decode_encode_instr_inv; eauto. }
+    { apply isCorrectPC_intro ; [solve_addr| auto]. }
+    { transitivity (Some ((b ^+ 14) ^+10)%a); solve_addr; done. }
+    { transitivity (Some a_m%a) ; solve_addr; done. }
+    iNext; iIntros "(HPC & Hi & Hr3 & Hr4)".
+    (* Close the invariant *)
+    iDestruct ("Hcont" with "Hi") as "Hprog".
+    iMod ("Hcls" with "Hprog") as "_".
+    simpl ; iModIntro ; wp_pure.
+
+    (* Mov *)
+    (* Open the invariant *)
+    wp_instr
+    ; iInv "Hinv_post" as ">Hprog" "Hcls"
+    (* Apply the invariant *)
+    ; iInstr_lookup "Hprog" as "Hi" "Hcont".
+    iApply ( wp_move_success_reg with "[ $HPC $Hr3 $Hr2 $Hi ]") ; eauto.
+    { cbn ;rewrite decode_encode_instr_inv; eauto. }
+    { apply isCorrectPC_intro ; [solve_addr| auto]. }
+    { transitivity (Some ((b ^+ 14) ^+11)%a); solve_addr; done. }
+    iNext; iIntros "(HPC & Hi & Hr3 & Hr2)".
+    (* Close the invariant *)
+    iDestruct ("Hcont" with "Hi") as "Hprog".
+    iMod ("Hcls" with "Hprog") as "_".
+    simpl ; iModIntro ; wp_pure.
+
+    (* sub *)
+    (* Open the invariant *)
+    wp_instr
+    ; iInv "Hinv_post" as ">Hprog" "Hcls"
+    (* Apply the invariant *)
+    ; iInstr_lookup "Hprog" as "Hi" "Hcont".
+    iApply ( wp_add_sub_lt_success_z_dst with "[ $HPC $Hr1 $Hi ]") ; eauto.
+    { rewrite decode_encode_instrW_inv ;cbn ; auto. }
+    { transitivity (Some ((b ^+ 14) ^+12)%a); solve_addr; done. }
+    { apply isCorrectPC_intro ; [solve_addr| auto]. }
+    iNext; iIntros "(HPC & Hi & Hr1)".
+    (* Close the invariant *)
+    iDestruct ("Hcont" with "Hi") as "Hprog".
+    iMod ("Hcls" with "Hprog") as "_".
+    simpl ; iModIntro ; wp_pure.
+    rewrite decode_encode_instr_inv /denote /=.
+    (* replace (a_m - (a_m ^+ size)%a)%Z with (-size)%Z by admit. *)
+
+
+    (* Lea *)
+    (* Open the invariant *)
+    wp_instr
+    ; iInv "Hinv_post" as ">Hprog" "Hcls"
+    (* Apply the invariant *)
+    ; iInstr_lookup "Hprog" as "Hi" "Hcont".
+    iApply ( wp_lea_success_reg with "[ $HPC $Hr3 $Hr1 $Hi ]") ; eauto.
+    { cbn ;rewrite decode_encode_instr_inv; eauto. }
+    { apply isCorrectPC_intro ; [solve_addr| auto]. }
+    { transitivity (Some ((b ^+ 14) ^+13)%a); solve_addr; done. }
+    { transitivity (Some 0%a) ; solve_addr; done. }
+    iNext; iIntros "(HPC & Hi & Hr1 & Hr3)".
+    (* Close the invariant *)
+    iDestruct ("Hcont" with "Hi") as "Hprog".
+    iMod ("Hcls" with "Hprog") as "_".
+    simpl ; iModIntro ; wp_pure.
+
+    (* GetB *)
+    (* Open the invariant *)
+    wp_instr
+    ; iInv "Hinv_post" as ">Hprog" "Hcls"
+    (* Apply the invariant *)
+    ; iInstr_lookup "Hprog" as "Hi" "Hcont".
+    iApply ( wp_Get_success with "[ $HPC $Hr1 $Hr3 $Hi ]") ; eauto.
+    { cbn ;rewrite decode_encode_instr_inv; eauto. }
+    { apply isCorrectPC_intro ; [solve_addr| auto]. }
+    { transitivity (Some ((b ^+ 14) ^+14)%a); solve_addr; done. }
+    iNext; iIntros "(HPC & Hi & Hr1 & Hr3)".
+    (* Close the invariant *)
+    iDestruct ("Hcont" with "Hi") as "Hprog".
+    iMod ("Hcls" with "Hprog") as "_".
+    simpl ; iModIntro ; wp_pure.
+    rewrite decode_encode_instr_inv /rules_Get.denote.
+
+
+    (* Lea *)
+    (* Open the invariant *)
+    wp_instr
+    ; iInv "Hinv_post" as ">Hprog" "Hcls"
+    (* Apply the invariant *)
+    ; iInstr_lookup "Hprog" as "Hi" "Hcont".
+    iApply ( wp_lea_success_reg with "[ $HPC $Hr3 $Hr1 $Hi ]") ; eauto.
+    { cbn ;rewrite decode_encode_instr_inv; eauto. }
+    { apply isCorrectPC_intro ; [solve_addr| auto]. }
+    { transitivity (Some ((b ^+ 14) ^+15)%a); solve_addr; done. }
+    { transitivity (Some b_m%a) ; solve_addr; done. }
+    iNext; iIntros "(HPC & Hi & Hr1 & Hr3)".
+    (* Close the invariant *)
+    iDestruct ("Hcont" with "Hi") as "Hprog".
+    iMod ("Hcls" with "Hprog") as "_".
+    simpl ; iModIntro ; wp_pure.
+
+    (* Store *)
+    (* Open the invariant *)
+    wp_instr
+    ; iInv "Hinv_post" as ">Hprog" "Hcls"
+    (* Apply the invariant *)
+    ; iInstr_lookup "Hprog" as "Hi" "Hcont".
+    iApply ( wp_store_success_reg with "[ $HPC $Hr2 $Hr3 $Hi $Hbm ]") ; eauto.
+    { cbn ;rewrite decode_encode_instr_inv; eauto. }
+    { apply isCorrectPC_intro ; [solve_addr| auto]. }
+    { transitivity (Some ((b ^+ 14) ^+16)%a); solve_addr; done. }
+    { solve_addr; done. }
+    iNext; iIntros "(HPC & Hi & Hr2 & Hr3 & Hbm)".
+    (* Close the invariant *)
+    iDestruct ("Hcont" with "Hi") as "Hprog".
+    iMod ("Hcls" with "Hprog") as "_".
+    simpl ; iModIntro ; wp_pure.
+
+    (* Mov *)
+    (* Open the invariant *)
+    wp_instr
+    ; iInv "Hinv_post" as ">Hprog" "Hcls"
+    (* Apply the invariant *)
+    ; iInstr_lookup "Hprog" as "Hi" "Hcont".
+    iApply ( wp_move_success_reg with "[ $HPC $Hr1 $Hr4 $Hi ]") ; eauto.
+    { cbn ;rewrite decode_encode_instr_inv; eauto. }
+    { apply isCorrectPC_intro ; [solve_addr| auto]. }
+    { transitivity (Some ((b ^+ 14) ^+17)%a); solve_addr; done. }
+    iNext; iIntros "(HPC & Hi & Hr1 & Hr4)".
+    (* Close the invariant *)
+    iDestruct ("Hcont" with "Hi") as "Hprog".
+    iMod ("Hcls" with "Hprog") as "_".
+    simpl ; iModIntro ; wp_pure.
+
+    (** --- release the lock --- *)
+    rewrite (region_addrs_zeroes_split _ (a_m ^+ size)%a)
+    ; [| solve_addr].
+    iDestruct (region_mapsto_split _ _ (a_m ^+ size)%a with "Hfree_reg")
+      as "[Hmem_fresh Hmem]".
+    solve_addr. by rewrite replicate_length //.
+
+    iApply (release_spec i _ _ _ _ r_t5 _ _ _ _ _ (* define P ? *) N E γ _
+             with "[-$HPC $Hlocked $Hr5]") ; auto.
+    { apply ExecPCPerm_RX. }
+    { solve_addr. }
+    { admit. }
+    Unshelve.
+    2: { exact (∃ b_m0 a_m0 : Addr,
+               ⌜(b + malloc_subroutine_instrs_length)%a = Some b_m0⌝
+                                                          ∗ b_m0 ↦ₐ WCap RWX b_m0 e a_m0
+                                                          ∗ [[a_m0,e]]↦ₐ[[region_addrs_zeroes a_m0 e]] ∗ ⌜(b_m0 < a_m0)%a ∧ (a_m0 <= e)%a⌝)%I.
+    }
+    iSplitR.
+    { iClear "Hinv_lock"
+      ; iClear "Hinv_pre"
+      ; iClear "Hinv_spin"
+      ; iClear "Hinv_post".
+
+    (* iDestruct (inv_split with "Hinv") as "[Hinv_code Hinv_lock]". *)
+    rewrite {1}/codefrag.
+    rewrite {1}/malloc_subroutine_instrs /malloc_subroutine_instrs'.
+    rewrite (region_mapsto_split _ _ (b ^+ malloc_pre_spin_length)%a).
+    2:{ cbn; rewrite /malloc_pre_spin_length; solve_addr. }
+    2:{ cbn; rewrite /malloc_pre_spin_length.
+        assert (H' : (b+8)%f = Some (b ^+8)%a) by solve_addr.
+        apply (finz_incr_iff_dist b (b ^+8)%a 8%nat) in H'.
+        destruct H' as [_ H'].
+        symmetry; apply H'. }
+    rewrite (region_mapsto_split (b ^+ malloc_pre_spin_length)%a _
+               ((b ^+ malloc_pre_spin_length ^+ spinlock_length)%a)).
+    2:{ rewrite /malloc_pre_spin_length /spinlock_length; solve_addr. }
+    2:{ cbn; rewrite /malloc_pre_spin_length /spinlock_length.
+        set (b' := (b ^+ 8)%a).
+        assert (H' : ((b ^+ 8)%a+6)%f = Some ((b ^+ 8)%a ^+6)%a) by solve_addr.
+        apply (finz_incr_iff_dist b' (b' ^+6)%a 6%nat) in H'.
+        destruct H' as [_ H'].
+        symmetry; apply H'. }
+    match goal with
+    | h: _ |- context [ is_lock ?g ?b ?P] => set (L := is_lock g b P)
+    end.
+    match goal with
+    | h: _ |- context [ region_mapsto ?b ?e ?l ] => set (P1 := region_mapsto b e l)
+    end.
+    match goal with
+    | h: _ |- context [ region_mapsto ?b ?e ?l ] => set (P2 := region_mapsto b e l)
+    end.
+    match goal with
+    | h: _ |- context [ region_mapsto ?b ?e ?l ] => set (P3 := region_mapsto b e l)
+    end.
+    match goal with
+    | h: _ |- context [ mapsto ?e ?d ?v ] => set (IE := mapsto e d v)
+    end.
+
+    subst P3. simpl.
+    replace (malloc_post_spin (malloc_subroutine_instrs_length - (5 + spinlock_length)))
+      with
+      (encodeInstrsW
+      [Mov r_t2 PC; Lea r_t2 (malloc_subroutine_instrs_length - (5 + spinlock_length))%Z;
+       Load r_t2 r_t2; GetA r_t3 r_t2; Lea r_t2 r_t1;
+       GetA r_t1 r_t2; Mov r_t4 r_t2; Subseg r_t4 r_t3 r_t1; Sub r_t3 r_t3 r_t1;
+       Lea r_t4 r_t3; Mov r_t3 r_t2; Sub r_t1 0%Z r_t1; Lea r_t3 r_t1; GetB r_t1 r_t3;
+       Lea r_t3 r_t1; Store r_t3 r_t2; Mov r_t1 r_t4]
+      ++ encodeInstrsW [Store r_t5 0]
+      ++
+      encodeInstrsW [Mov r_t2 0%Z;
+                     Mov r_t3 0%Z; Mov r_t4 0%Z; Mov r_t5 0%Z; Mov r_t6 0%Z; Mov r_t7 0%Z; Mov r_t8 0%Z;
+                     Jmp r_t0])
+    by (rewrite /malloc_post_spin ; auto).
+    rewrite (region_mapsto_split ((b ^+ malloc_pre_spin_length) ^+ spinlock_length)%a _
+               ((b ^+ 14) ^+ 17)%a ).
+    2:{ rewrite /malloc_pre_spin_length /spinlock_length; solve_addr. }
+    2:{ cbn; rewrite /malloc_pre_spin_length /spinlock_length.
+        replace ( ((b ^+ 8) ^+ 6)%a ) with ((b ^+ 14))%a by solve_addr.
+        set (b' := (b ^+ 14)%a).
+        assert (H' : ((b ^+ 14)%a+17)%f = Some ((b ^+ 14)%a ^+17)%a) by solve_addr.
+        apply (finz_incr_iff_dist b' (b' ^+17)%a 17%nat) in H'.
+        destruct H' as [_ H'].
+        symmetry; apply H'. }
+
+    rewrite (region_mapsto_split ((b ^+ 14) ^+ 17)%a _
+               ((b ^+ 14) ^+ 18)%a ).
+    2:{ solve_addr. }
+    2:{ cbn.
+        replace ((b ^+ 14) ^+ 17)%a with ((b ^+ 31))%a by solve_addr.
+        replace ((b ^+ 14) ^+ 18)%a with ((b ^+ 31) ^+1)%a by solve_addr.
+        rewrite finz_dist_S ; last solve_addr.
+        rewrite finz_dist_0 ; last solve_addr.
+        done. }
+    match goal with
+    | h: _ |- context [ region_mapsto ?b ?e ?l ] => set (P3 := region_mapsto b e l)
+    end.
+    match goal with
+    | h: _ |- context [ region_mapsto ?b ?e ?l ] => set (P4 := region_mapsto b e l)
+    end.
+    match goal with
+    | h: _ |- context [ region_mapsto ?b ?e ?l ] => set (P5 := region_mapsto b e l)
+    end.
+    iAssert ( inv N ( (P4 ∗ L) ∗ (P1 ∗ P2 ∗ P3 ∗ P5) ∗ IE ) ) as "Hinv1".
+    iApply (inv_iff with "[$Hinv]")
+     ; first (do 2 iModIntro ; iSplit ;
+              [iIntros "((?&?&?&?&?) & ? & ?)" | iIntros "((? & ?) & (?&?&?&?) & ?)" ]
+               ; iFrame).
+    iDestruct (inv_split_l with "Hinv1") as "Hinv2".
+    iClear "Hinv" ; iClear "Hinv1" ; clear -P4.
+    assert (P4 =  codefrag ((b ^+ 14) ^+ 17)%a [encodeInstrW (Store r_t5 0)]).
+    { subst P4. rewrite /codefrag /=.
+      replace (((b ^+ 14) ^+ 17) ^+ 1%nat)%a with ((b ^+ 14) ^+ 18)%a by solve_addr.
+      done. }
+    rewrite H0.
+    iFrame "Hinv2".
+    }
+
+    iSplitL "Hbm Hmem".
+    iExists b_m , (a_m^+size)%a.
+    replace a_m' with (a_m ^+size)%a by solve_addr.
+    iFrame "∗%".
+    iPureIntro. solve_addr.
+    iNext; iIntros "(HPC & Hr5)".
+    replace (((b ^+ 14) ^+ 17) ^+ 1)%a with (((b ^+ 14) ^+ 18)%a) by solve_addr.
+
+    (* Mov *)
+    (* Open the invariant *)
+    wp_instr
+    ; iInv "Hinv_post" as ">Hprog" "Hcls"
+    (* Apply the invariant *)
+    ; iInstr_lookup "Hprog" as "Hi" "Hcont".
+    iApply ( wp_move_success_z with "[ $HPC $Hr2 $Hi ]") ; eauto.
+    { cbn ;rewrite decode_encode_instr_inv; eauto. }
+    { apply isCorrectPC_intro ; [solve_addr| auto]. }
+    { transitivity (Some ((b ^+ 14) ^+19)%a); solve_addr; done. }
     iNext; iIntros "(HPC & Hi & Hr2)".
     (* Close the invariant *)
     iDestruct ("Hcont" with "Hi") as "Hprog".
     iMod ("Hcls" with "Hprog") as "_".
     simpl ; iModIntro ; wp_pure.
 
+
+
     (* Mov *)
     (* Open the invariant *)
     wp_instr
-    ; iInv "Hinv_pre" as ">Hprog" "Hcls"
-    ; codefrag_facts "Hprog".
+    ; iInv "Hinv_post" as ">Hprog" "Hcls"
     (* Apply the invariant *)
-    iInstr_lookup "Hprog" as "Hi" "Hcont"
-    ; iApply ( wp_move_success_reg_fromPC with "[ $HPC $Hr5 $Hi ]") ; eauto.
+    ; iInstr_lookup "Hprog" as "Hi" "Hcont".
+    iApply ( wp_move_success_z with "[ $HPC $Hr3 $Hi ]") ; eauto.
     { cbn ;rewrite decode_encode_instr_inv; eauto. }
     { apply isCorrectPC_intro ; [solve_addr| auto]. }
-    { transitivity (Some (b ^+ 7)%a); solve_addr; done. }
-    iNext; iIntros "(HPC & Hi & Hr5)".
+    { transitivity (Some ((b ^+ 14) ^+20)%a); solve_addr; done. }
+    iNext; iIntros "(HPC & Hi & Hr3)".
     (* Close the invariant *)
     iDestruct ("Hcont" with "Hi") as "Hprog".
     iMod ("Hcls" with "Hprog") as "_".
     simpl ; iModIntro ; wp_pure.
 
-    (* Lea *)
+    (* Mov *)
     (* Open the invariant *)
     wp_instr
-    ; iInv "Hinv_pre" as ">Hprog" "Hcls"
-    ; codefrag_facts "Hprog".
+    ; iInv "Hinv_post" as ">Hprog" "Hcls"
     (* Apply the invariant *)
-    iInstr_lookup "Hprog" as "Hi" "Hcont"
-    ; iApply ( wp_lea_success_z with "[ $HPC $Hr5 $Hi ]") ; eauto.
+    ; iInstr_lookup "Hprog" as "Hi" "Hcont".
+    iApply ( wp_move_success_z with "[ $HPC $Hr4 $Hi ]") ; eauto.
     { cbn ;rewrite decode_encode_instr_inv; eauto. }
     { apply isCorrectPC_intro ; [solve_addr| auto]. }
-    { transitivity (Some (b ^+ 8)%a); solve_addr; done. }
-    { rewrite /malloc_subroutine_instrs_length.
-      transitivity (Some (b ^+ 41)%a).
-      rewrite (_ : (39 - 5 + 1) = 35 )%Z ; last lia.
-      admit. done. }
+    { transitivity (Some ((b ^+ 14) ^+21)%a); solve_addr; done. }
+    iNext; iIntros "(HPC & Hi & Hr4)".
+    (* Close the invariant *)
+    iDestruct ("Hcont" with "Hi") as "Hprog".
+    iMod ("Hcls" with "Hprog") as "_".
+    simpl ; iModIntro ; wp_pure.
+
+    (* Mov *)
+    (* Open the invariant *)
+    wp_instr
+    ; iInv "Hinv_post" as ">Hprog" "Hcls"
+    (* Apply the invariant *)
+    ; iInstr_lookup "Hprog" as "Hi" "Hcont".
+    iApply ( wp_move_success_z with "[ $HPC $Hr5 $Hi ]") ; eauto.
+    { cbn ;rewrite decode_encode_instr_inv; eauto. }
+    { apply isCorrectPC_intro ; [solve_addr| auto]. }
+    { transitivity (Some ((b ^+ 14) ^+22)%a); solve_addr; done. }
     iNext; iIntros "(HPC & Hi & Hr5)".
     (* Close the invariant *)
     iDestruct ("Hcont" with "Hi") as "Hprog".
     iMod ("Hcls" with "Hprog") as "_".
     simpl ; iModIntro ; wp_pure.
 
-    (* TODO: I need to extract the address of the lock, in order to give it to
-             the spec, but it depends on the existantial b_m..... Find a solution *)
-    (** ====== Spinlock ====== *)
-    iApply (spinlock_spec i _ _ _ _ r_t5 r_t6 r_t7 r_t8 with "[$HPC $Hr5 $Hr6 $Hr7 $Hr8]").
-    { apply ExecPCPerm_RX. }
-    { solve_addr. }
-    { admit. }
-    { admit. }
-    { eauto. }
-    iFrame "#".
-Abort.
+    (* Mov *)
+    (* Open the invariant *)
+    wp_instr
+    ; iInv "Hinv_post" as ">Hprog" "Hcls"
+    (* Apply the invariant *)
+    ; iInstr_lookup "Hprog" as "Hi" "Hcont".
+    iApply ( wp_move_success_z with "[ $HPC $Hr6 $Hi ]") ; eauto.
+    { cbn ;rewrite decode_encode_instr_inv; eauto. }
+    { apply isCorrectPC_intro ; [solve_addr| auto]. }
+    { transitivity (Some ((b ^+ 14) ^+23)%a); solve_addr; done. }
+    iNext; iIntros "(HPC & Hi & Hr6)".
+    (* Close the invariant *)
+    iDestruct ("Hcont" with "Hi") as "Hprog".
+    iMod ("Hcls" with "Hprog") as "_".
+    simpl ; iModIntro ; wp_pure.
+
+    (* Mov *)
+    (* Open the invariant *)
+    wp_instr
+    ; iInv "Hinv_post" as ">Hprog" "Hcls"
+    (* Apply the invariant *)
+    ; iInstr_lookup "Hprog" as "Hi" "Hcont".
+    iDestruct "Hr7" as (w7) "Hr7".
+    iApply ( wp_move_success_z with "[ $HPC $Hr7 $Hi ]") ; eauto.
+    { cbn ;rewrite decode_encode_instr_inv; eauto. }
+    { apply isCorrectPC_intro ; [solve_addr| auto]. }
+    { transitivity (Some ((b ^+ 14) ^+24)%a); solve_addr; done. }
+    iNext; iIntros "(HPC & Hi & Hr7)".
+    (* Close the invariant *)
+    iDestruct ("Hcont" with "Hi") as "Hprog".
+    iMod ("Hcls" with "Hprog") as "_".
+    simpl ; iModIntro ; wp_pure.
+
+    (* Mov *)
+    (* Open the invariant *)
+    wp_instr
+    ; iInv "Hinv_post" as ">Hprog" "Hcls"
+    (* Apply the invariant *)
+    ; iInstr_lookup "Hprog" as "Hi" "Hcont".
+    iApply ( wp_move_success_z with "[ $HPC $Hr8 $Hi ]") ; eauto.
+    { cbn ;rewrite decode_encode_instr_inv; eauto. }
+    { apply isCorrectPC_intro ; [solve_addr| auto]. }
+    { transitivity (Some ((b ^+ 14) ^+25)%a); solve_addr; done. }
+    iNext; iIntros "(HPC & Hi & Hr8)".
+    (* Close the invariant *)
+    iDestruct ("Hcont" with "Hi") as "Hprog".
+    iMod ("Hcls" with "Hprog") as "_".
+    simpl ; iModIntro ; wp_pure.
+
+
+    (* Jmp *)
+    (* Open the invariant *)
+    wp_instr
+    ; iInv "Hinv_post" as ">Hprog" "Hcls"
+    (* Apply the invariant *)
+    ; iInstr_lookup "Hprog" as "Hi" "Hcont".
+    iApply ( wp_jmp_success with "[ $HPC $Hr0 $Hi ]") ; eauto.
+    { cbn ;rewrite decode_encode_instr_inv; eauto. }
+    { apply isCorrectPC_intro ; [solve_addr| auto]. }
+    iNext; iIntros "(HPC & Hi & Hr0)".
+    (* Close the invariant *)
+    iDestruct ("Hcont" with "Hi") as "Hprog".
+    iMod ("Hcls" with "Hprog") as "_".
+    simpl ; iModIntro ; wp_pure.
+
+
+    iApply (wp_wand with "[-]").
+    { iApply "Hφ". iFrame.
+      iDestruct (big_sepM_insert with "[$Hrmap $Hr8]") as "Hrmap".
+      by rewrite lookup_delete. rewrite insert_delete.
+      iDestruct (big_sepM_insert with "[$Hrmap $Hr7]") as "Hrmap".
+      rewrite !lookup_insert_ne ;
+        [by rewrite lookup_delete | simplify_pair_eq].
+      iDestruct (big_sepM_insert with "[$Hrmap $Hr6]") as "Hrmap".
+      rewrite !lookup_insert_ne ; [ | simplify_pair_eq | simplify_pair_eq].
+      rewrite lookup_delete_ne  ; [ | simplify_pair_eq ].
+      by rewrite lookup_delete.
+      iDestruct (big_sepM_insert with "[$Hrmap $Hr5]") as "Hrmap".
+      rewrite !lookup_insert_ne ; [ | simplify_pair_eq
+                                    | simplify_pair_eq
+                                    | simplify_pair_eq].
+      do 2 (rewrite lookup_delete_ne  ; [ |simplify_pair_eq]).
+      by rewrite lookup_delete.
+      iDestruct (big_sepM_insert with "[$Hrmap $Hr4]") as "Hrmap".
+      rewrite !lookup_insert_ne ; [ | simplify_pair_eq
+                                    | simplify_pair_eq
+                                    | simplify_pair_eq
+                                    | simplify_pair_eq].
+      do 3 (rewrite lookup_delete_ne  ; [ |simplify_pair_eq]).
+      by rewrite lookup_delete.
+      iDestruct (big_sepM_insert with "[$Hrmap $Hr3]") as "Hrmap".
+      rewrite !lookup_insert_ne ; [ | simplify_pair_eq
+                                    | simplify_pair_eq
+                                    | simplify_pair_eq
+                                    | simplify_pair_eq
+                                    | simplify_pair_eq].
+      do 4 (rewrite lookup_delete_ne  ; [ |simplify_pair_eq]).
+      by rewrite lookup_delete.
+      iDestruct (big_sepM_insert with "[$Hrmap $Hr2]") as "Hrmap".
+      rewrite !lookup_insert_ne ; [ | simplify_pair_eq
+                                    | simplify_pair_eq
+                                    | simplify_pair_eq
+                                    | simplify_pair_eq
+                                    | simplify_pair_eq
+                                    | simplify_pair_eq].
+      do 5 (rewrite lookup_delete_ne  ; [ |simplify_pair_eq]).
+      by rewrite lookup_delete.
+      iSplitL "Hrmap".
+      { rewrite (insert_commute _ (i, r_t7) (i, r_t8)) ; last simplify_pair_eq.
+        rewrite insert_delete.
+        do 2 (rewrite (insert_commute _ (i, r_t6) _) ; last simplify_pair_eq).
+        rewrite insert_delete.
+        do 3 (rewrite (insert_commute _ (i, r_t5) _) ; last simplify_pair_eq).
+        rewrite insert_delete.
+        do 4 (rewrite (insert_commute _ (i, r_t4) _) ; last simplify_pair_eq).
+        rewrite insert_delete.
+        do 5 (rewrite (insert_commute _ (i, r_t3) _) ; last simplify_pair_eq).
+        rewrite insert_delete.
+        do 6 (rewrite (insert_commute _ (i, r_t2) _) ; last simplify_pair_eq).
+        rewrite insert_delete.
+        do 6 (rewrite (insert_commute _ (i, r_t8) _) ; last simplify_pair_eq).
+        do 5 (rewrite (insert_commute _ (i, r_t7) _) ; last simplify_pair_eq).
+        do 4 (rewrite (insert_commute _ (i, r_t6) _) ; last simplify_pair_eq).
+        do 3 (rewrite (insert_commute _ (i, r_t5) _) ; last simplify_pair_eq).
+        do 2 (rewrite (insert_commute _ (i, r_t4) _) ; last simplify_pair_eq).
+        rewrite (insert_commute _ (i, r_t3) _) ; last simplify_pair_eq.
+        iFrame. }
+      iExists a_m, a_m', size.
+      replace (a_m ^+ size)%a with a_m' by solve_addr.
+      iFrame.
+      iSplit ; eauto.
+    }
+      iIntros (v) "Hφ" ; iLeft ; done.
+Admitted.
+
+
 
 
 
